ITree_Extraction.thy
@@ -1,7 +1,7 @@
 subsection \<open> ITree Code Generation Support \<close>
 
 theory ITree_Extraction
-  imports ITree_Circus Record_Default_Instance
+  imports ITree_Circus Record_Default_Instance Enum_Type
 begin
 
 instantiation set :: (type) default
